ctl: implement IsEquiv for Equiv

CTL/Equivalence.lean
@@ -4,18 +4,19 @@ import CTL.Satisfaction
 
 namespace CTL
 variable {p : Type}
-         (Φ Ψ : @StateFormula p)
+         {Φ Φ' Ψ Ψ' : @StateFormula p}
 
 -- Sat(Φ) = Sat(Ψ)
 @[simp]
-def Equiv :=
+def Equiv (Φ Ψ : @StateFormula p) :=
   ∀{s a : Type} , ∀{ts : @TS s a p}, satStateSet ts Φ = satStateSet ts Ψ
 
 -- TS ⊨ Φ ↔ TS ⊨ Ψ
 @[simp]
-def Equiv' :=
+def Equiv' (Φ Ψ : @StateFormula p) :=
   ∀{s a : Type} , ∀{ts : @TS s a p}, Sat ts Φ ↔ Sat ts Ψ
 
+namespace Equiv
 @[simp]
 theorem equiv'_of_equiv : Equiv Φ Ψ → Equiv' Φ Ψ := by
   simp [Equiv, Equiv']
@@ -23,8 +24,21 @@ theorem equiv'_of_equiv : Equiv Φ Ψ → Equiv' Φ Ψ := by
   rewrite [h]
   trivial
 
+instance : IsRefl (@StateFormula p) Equiv where
+  refl := by simp
+
+instance : IsSymm (@StateFormula p) Equiv where
+  symm := fun Φ Ψ => by simp; intros h _ _ _; exact Eq.symm h
+
+instance : IsTrans (@StateFormula p) Equiv where
+  trans := fun _ _ _ h₁ h₂ => Trans.trans h₁ h₂
+
+instance : IsPreorder (@StateFormula p) Equiv where
+
+instance : IsEquiv (@StateFormula p) Equiv where
+
 @[simp]
-theorem equiv_conj_congr (h₁ : Equiv Φ₁ Φ₁') (h₂ : Equiv Φ₂ Φ₂') : Equiv (Φ₁ ⬝∧ Φ₂) (Φ₁' ⬝∧ Φ₂') := by
+theorem conj_congr (h₁ : Equiv Φ₁ Φ₁') (h₂ : Equiv Φ₂ Φ₂') : Equiv (Φ₁ ⬝∧ Φ₂) (Φ₁' ⬝∧ Φ₂') := by
   simp [Equiv, satStateSet, SatState, StateSat, Set.ext_iff] at *
   intros _ _ _ _
   constructor
@@ -32,7 +46,7 @@ theorem equiv_conj_congr (h₁ : Equiv Φ₁ Φ₁') (h₂ : Equiv Φ₂ Φ₂')
   . rintro ⟨sat₁, sat₂⟩; constructor; exact (h₁ _).2 sat₁; exact (h₂ _).2 sat₂
 
 @[simp]
-theorem equiv_neg_congr (h : Equiv Φ Φ') : Equiv (⬝¬Φ) (⬝¬Φ') := by
+theorem neg_congr (h : Equiv Φ Φ') : Equiv (⬝¬Φ) (⬝¬Φ') := by
   simp [Equiv, satStateSet, SatState, StateSat, Set.ext_iff] at *
   intros _ _ _ _
   constructor
@@ -40,7 +54,7 @@ theorem equiv_neg_congr (h : Equiv Φ Φ') : Equiv (⬝¬Φ) (⬝¬Φ') := by
   . rintro negSat sat; exact negSat ((h _).1 sat)
 
 @[simp]
-theorem equiv_exist_next_congr (h : Equiv Φ Φ') : Equiv (⬝∃⬝◯Φ) (⬝∃⬝◯Φ') := by
+theorem exist_next_congr (h : Equiv Φ Φ') : Equiv (⬝∃⬝◯Φ) (⬝∃⬝◯Φ') := by
   simp [Equiv, satStateSet, SatState, StateSat, PathSat, Set.ext_iff] at *
   intros _ _ _ _
   constructor
@@ -48,7 +62,7 @@ theorem equiv_exist_next_congr (h : Equiv Φ Φ') : Equiv (⬝∃⬝◯Φ) (⬝�
   . rintro ⟨π, sat⟩; exact ⟨π, (h _).2 sat⟩
 
 @[simp]
-theorem equiv_exist_untl_congr (h₁ : Equiv Φ Φ') (h₂ : Equiv Ψ Ψ') : Equiv (⬝∃(Φ ⬝U Ψ)) (⬝∃(Φ' ⬝U Ψ')) := by
+theorem exist_untl_congr (h₁ : Equiv Φ Φ') (h₂ : Equiv Ψ Ψ') : Equiv (⬝∃(Φ ⬝U Ψ)) (⬝∃(Φ' ⬝U Ψ')) := by
   simp [Equiv, satStateSet, SatState, StateSat, PathSat, Set.ext_iff] at *
   intros _ _ _ _
   constructor
@@ -56,7 +70,7 @@ theorem equiv_exist_untl_congr (h₁ : Equiv Φ Φ') (h₂ : Equiv Ψ Ψ') : Equ
   . rintro ⟨π, j, ⟨satJ, satK⟩⟩; exact ⟨π, j, ⟨(h₂ _).2 satJ, fun k => (h₁ _).2 (satK k)⟩⟩
 
 @[simp]
-theorem equiv_all_next_congr (h : Equiv Φ Φ') : Equiv (⬝∀⬝◯Φ) (⬝∀⬝◯Φ') := by
+theorem all_next_congr (h : Equiv Φ Φ') : Equiv (⬝∀⬝◯Φ) (⬝∀⬝◯Φ') := by
   simp [Equiv, satStateSet, SatState, StateSat, PathSat, Set.ext_iff] at *
   intros _ _ _ _
   constructor
@@ -65,7 +79,7 @@ theorem equiv_all_next_congr (h : Equiv Φ Φ') : Equiv (⬝∀⬝◯Φ) (⬝∀
   done
 
 @[simp]
-theorem equiv_all_untl_congr (h₁ : Equiv Φ Φ') (h₂ : Equiv Ψ Ψ') : Equiv (⬝∀(Φ ⬝U Ψ)) (⬝∀(Φ' ⬝U Ψ')) := by
+theorem all_untl_congr (h₁ : Equiv Φ Φ') (h₂ : Equiv Ψ Ψ') : Equiv (⬝∀(Φ ⬝U Ψ)) (⬝∀(Φ' ⬝U Ψ')) := by
   simp [Equiv, satStateSet, SatState, StateSat, PathSat, Set.ext_iff] at *
   intros _ _ _ _
   constructor
@@ -93,5 +107,6 @@ theorem all_untl_expansion : Equiv (⬝∀(Φ ⬝U Ψ)) (Ψ ⬝∨ (Φ ⬝∧ (�
   -- ext x
   -- done
   sorry
+end Equiv
 
 end CTL
